wip

Logic/Vorspiel/Vorspiel.lean
@@ -823,5 +823,5 @@ lemma subset_tetraunion₂ : s₂ ⊆ (s₁ ∪ s₂ ∪ s₃ ∪ s₄) :=
 end Set
 
 /-- Class for `α` has at least `n` elements -/
-class Atleast (n : ℕ+) (α) where
+class AtLeast (n : ℕ+) (α) where
   mapping : ∃ f : Fin n → α, Function.HasLeftInverse f
